src/syntax/print.fs
@@ -235,7 +235,7 @@ let rec term_to_string x =
         | Some (Inl l) when (Options.print_implicits()) -> 
           Util.format3 "(fun %s -> (%s $$ %s))" (binders_to_string " " bs) (term_to_string t2) (comp_to_string <| l.comp())
         | Some (Inr l) when (Options.print_implicits()) -> 
-          Util.format3 "(fun %s -> (%s $$ %s))" (binders_to_string " " bs) (term_to_string t2) l.str
+          Util.format3 "(fun %s -> (%s $$ (name only) %s))" (binders_to_string " " bs) (term_to_string t2) l.str
         | _ -> 
           Util.format2 "(fun %s -> %s)" (binders_to_string " " bs) (term_to_string t2)
     end
