examples/dm4free/natST.fst
@@ -6,7 +6,10 @@ let st_wp (a:Type) = int -> st_post a -> Type0
 assume val r0: range
 inline let st_return_wp (a:Type) (x:a) (n0:int) (post:st_post a) = 
   forall y. y=(x, n0) ==> post y
-inline let st_bind_wp (r:range) (a:Type) (b:Type) (f:st_wp a) (g:(a -> Tot (st_wp b))) : st_wp b = 
+
+//working around #517 by adding an explicit 'val'
+inline val st_bind_wp : r:range -> (a:Type) -> (b:Type) -> (f:st_wp a) -> (g:(a -> Tot (st_wp b))) -> Tot (st_wp b)
+let st_bind_wp r a b f g =
     fun n0 post -> f n0 (fun x_n1 -> g (fst x_n1) (snd x_n1) post)
 
 inline let st_if_then_else  (a:Type) (p:Type)
@@ -44,24 +47,26 @@ inline let st_trivial       (a:Type)
      (forall h0. wp h0 (fun r -> True))
 
 //new
-let st_repr (a:Type) (wp:st_wp a) =  
+let st_repr (a:Type) (wp:st_wp a) =
     n0:int -> PURE (a * int) (wp n0)
-inline let st_bind (r:range) (a:Type) (b:Type) (wp0:st_wp a) (wp1:(a -> Tot (st_wp b)))
-	    (f:st_repr a wp0)
-	    (g:(x:a -> Tot (st_repr b (wp1 x)))) 
-  : st_repr b (st_bind_wp r a b wp0 wp1)
-  = fun n0 -> admit(); let x, n1 = f n0 in g x n1
-let st_return (a:Type) (x:a) 
+
+inline val st_bind: (a:Type) -> (b:Type) -> (wp0:st_wp a) -> (wp1:(a -> Tot (st_wp b))) 
+		 -> (f:st_repr a wp0)
+		 -> (g:(x:a -> Tot (st_repr b (wp1 x)))) 
+		 -> Tot (st_repr b (st_bind_wp r0 a b wp0 wp1))
+let st_bind a b wp0 wp1 f g  
+  = fun n0 -> admit(); let (x,n1) = f n0 in g x n1
+let st_return (a:Type) (x:a)
   : st_repr a (st_return_wp a x)
   = fun n0 -> (x, n0)
 
-let st_get (u:unit) : st_repr int (fun n0 post -> post (n0, n0)) 
+let st_get (u:unit) : st_repr int (fun n0 post -> post (n0, n0))
   = fun n0 -> n0, n0
 
 let st_put (n:int) : st_repr unit (fun n0 post -> post ((), n))
   = fun x -> (), n
 
-//#reset-options "--debug NatST --debug_level SMTEncoding"
+(* //#reset-options "--debug NatST --debug_level SMTEncoding" *)
 
 reifiable reflectable new_effect {
   STATE : a:Type -> wp:st_wp a -> Effect
@@ -93,7 +98,7 @@ reifiable reflectable new_effect {
 inline let lift_pure_state (a:Type) (wp:pure_wp a) (n:int) (p:st_post a) = wp (fun a -> p (a, n))
 sub_effect PURE ~> STATE = lift_pure_state
 
-effect ST (a:Type) (pre:st_pre) (post: (int -> a -> int -> GTot Type0)) = 
+effect ST (a:Type) (pre:st_pre) (post: (int -> a -> int -> GTot Type0)) =
        STATE a
              (fun n0 p -> pre n0 /\ (forall a n1. pre n0 /\ post n0 a n1 ==> p (a, n1)))
 
@@ -103,102 +108,102 @@ effect St (a:Type) =
 
 ////////////////////////////////////////////////////////////////////////////////
 
-val incr : unit -> ST unit (requires (fun n -> True))
-			  (ensures (fun n0 _ n1 -> n1 = n0 + 1))
-let incr u = 
-  let n = STATE.get () in
-  STATE.put (n + 1)
+(* val incr : unit -> ST unit (requires (fun n -> True)) *)
+(* 			  (ensures (fun n0 _ n1 -> n1 = n0 + 1)) *)
+(* let incr u = *)
+(*   let n = STATE.get () in *)
+(*   STATE.put (n + 1) *)
 
-reifiable val incr2 : unit -> St unit
-let incr2 u =
-    let n = STATE.get() in
-    STATE.put (n + 1)
+(* reifiable val incr2 : unit -> St unit *)
+(* let incr2 u = *)
+(*     let n = STATE.get() in *)
+(*     STATE.put (n + 1) *)
 
-(* #set-options "--log_queries" *)
-module Test
-open NatST
-let f (_:unit) : St unit =
-    let n0 = STATE.get() in
-    let _, n1 = reify (incr2 ()) n0 in
-    assert (n1 = n0 + 1);
-    STATE.put n1
+(* (\* #set-options "--log_queries" *\) *)
+(* module Test *)
+(* open NatST *)
+(* let f (_:unit) : St unit = *)
+(*     let n0 = STATE.get() in *)
+(*     let _, n1 = reify (incr2 ()) n0 in *)
+(*     assert (n1 = n0 + 1); *)
+(*     STATE.put n1 *)
 
-val g : unit -> St int
-let g u =
-    let n0 = STATE.get () in
-    let f : st_repr unit (fun n0 post -> forall x. snd x=n0+2 ==> post x) =
-      fun n0 -> (), n0+2 in
-    STATE.reflect f;
-    let n1 = STATE.get () in
-    assert (n0 + 2 = n1);
-    n1
+(* val g : unit -> St int *)
+(* let g u = *)
+(*     let n0 = STATE.get () in *)
+(*     let f : st_repr unit (fun n0 post -> forall x. snd x=n0+2 ==> post x) = *)
+(*       fun n0 -> (), n0+2 in *)
+(*     STATE.reflect f; *)
+(*     let n1 = STATE.get () in *)
+(*     assert (n0 + 2 = n1); *)
+(*     n1 *)
 
     
     
 
 
-(* sub_effect PURE ~> STATE { *)
-(*   lift_wp: #a:Type -> #wp:pure_wp a -> st_wp a = ... *)
-(*   lift   : #a:Type -> #wp:pure_wp a -> f:PURE.repr a wp -> STATE.repr a (lift_star wp) = ... *)
-(* }   *)
+(* (\* sub_effect PURE ~> STATE { *\) *)
+(* (\*   lift_wp: #a:Type -> #wp:pure_wp a -> st_wp a = ... *\) *)
+(* (\*   lift   : #a:Type -> #wp:pure_wp a -> f:PURE.repr a wp -> STATE.repr a (lift_star wp) = ... *\) *)
+(* (\* }   *\) *)
 
-(* //////////////////////////////////////////////////////////////////////////////// *)
-(* (\* let repr_STATE (a:Type) (wp:st_wp a) =  *\) *)
-(* (\*   n0:nat -> PURE (a * nat) (fun post -> wp (fun a n -> post (a, n)) n0) *\) *)
-
-
-
-(* new_effect STATE = STATE_h nat *)
-(* let st_pre = st_pre_h nat *)
-(* let st_post a = st_post_h nat a *)
-(* let st_wp a = st_wp_h nat a *)
-(* inline let lift_pure_state (a:Type) (wp:pure_wp a) (p:st_post a) (n:nat) = wp (fun a -> p a n) *)
-(* sub_effect PURE ~> STATE = lift_pure_state *)
-
-(* let reify_STATE (a:Type) = nat -> Tot (a * nat) *)
-(* let reify_return (#a:Type) (x:a) : reify_STATE a = fun n -> (x, n) *)
-(* let reify_bind (#a:Type) (#b:Type) (f:reify_STATE a) (g:(a -> Tot (reify_STATE b)) ) *)
-(*   : reify_STATE b  *)
-(*   = fun n0 -> let x, n1 = f n0 in g x n1 *)
-(* let reify_get () : reify_STATE nat =  *)
-(*   fun n -> n, n *)
-(* let reify_put (m:nat) : reify_STATE unit =  *)
-(*  fun _ -> (), m *)
-
-(* assume val get : unit -> STATE nat (fun post n -> post n n) *)
-(* assume val put : m:nat -> STATE unit (fun post n -> post () m) *)
-
-(* val incr : unit -> STATE unit (fun post n -> post () (n + 1)) *)
-(* let incr () =  *)
-(*   let n = get () in  *)
-(*   put (n + 1) *)
-
-(* val incr2 : unit -> STATE unit (fun post n -> forall m. post () m) *)
-(* let incr2 () =  *)
-(*   let n = get () in  *)
-(*   put (n + 1) *)
+(* (\* //////////////////////////////////////////////////////////////////////////////// *\) *)
+(* (\* (\\* let repr_STATE (a:Type) (wp:st_wp a) =  *\\) *\) *)
+(* (\* (\\*   n0:nat -> PURE (a * nat) (fun post -> wp (fun a n -> post (a, n)) n0) *\\) *\) *)
 
 
 
-
-
-
-(* (\* let repr_STATE (a:Type) (wp:st_wp a) =  *\) *)
-(* (\*   n0:nat -> PURE (a * nat) (fun post -> wp (fun a n -> post (a, n)) n0) *\) *)
-
+(* (\* new_effect STATE = STATE_h nat *\) *)
+(* (\* let st_pre = st_pre_h nat *\) *)
+(* (\* let st_post a = st_post_h nat a *\) *)
+(* (\* let st_wp a = st_wp_h nat a *\) *)
 (* (\* inline let lift_pure_state (a:Type) (wp:pure_wp a) (p:st_post a) (n:nat) = wp (fun a -> p a n) *\) *)
 (* (\* sub_effect PURE ~> STATE = lift_pure_state *\) *)
-(* (\* assume val r : range *\) *)
 
-(* (\* val repr_bind: #a:Type -> #b:Type -> #wp1:st_wp a -> #wp2:(a -> GTot (st_wp b)) *\) *)
-(* (\* 	     -> repr_STATE a wp1 *\) *)
-(* (\* 	     -> (x:a -> Tot (repr_STATE b (wp2 x))) *\) *)
-(* (\* 	     -> Tot (repr_STATE b (st_bind_wp nat r a b wp1 wp2)) *\) *)
-(* (\* #reset-options "--log_queries"	      *\) *)
-(* (\* let repr_bind #a #b #wp1 #wp2 f g =  *\) *)
-(* (\*   fun n0 -> admit(); //the encoding to SMT isn't sufficiently smart to capture monotonicity *\) *)
-(* (\*          let x, n1 = f n0 in *\) *)
-(* (\*          g x n1 *\) *)
+(* (\* let reify_STATE (a:Type) = nat -> Tot (a * nat) *\) *)
+(* (\* let reify_return (#a:Type) (x:a) : reify_STATE a = fun n -> (x, n) *\) *)
+(* (\* let reify_bind (#a:Type) (#b:Type) (f:reify_STATE a) (g:(a -> Tot (reify_STATE b)) ) *\) *)
+(* (\*   : reify_STATE b  *\) *)
+(* (\*   = fun n0 -> let x, n1 = f n0 in g x n1 *\) *)
+(* (\* let reify_get () : reify_STATE nat =  *\) *)
+(* (\*   fun n -> n, n *\) *)
+(* (\* let reify_put (m:nat) : reify_STATE unit =  *\) *)
+(* (\*  fun _ -> (), m *\) *)
+
+(* (\* assume val get : unit -> STATE nat (fun post n -> post n n) *\) *)
+(* (\* assume val put : m:nat -> STATE unit (fun post n -> post () m) *\) *)
+
+(* (\* val incr : unit -> STATE unit (fun post n -> post () (n + 1)) *\) *)
+(* (\* let incr () =  *\) *)
+(* (\*   let n = get () in  *\) *)
+(* (\*   put (n + 1) *\) *)
+
+(* (\* val incr2 : unit -> STATE unit (fun post n -> forall m. post () m) *\) *)
+(* (\* let incr2 () =  *\) *)
+(* (\*   let n = get () in  *\) *)
+(* (\*   put (n + 1) *\) *)
+
+
+
+
+
+
+(* (\* (\\* let repr_STATE (a:Type) (wp:st_wp a) =  *\\) *\) *)
+(* (\* (\\*   n0:nat -> PURE (a * nat) (fun post -> wp (fun a n -> post (a, n)) n0) *\\) *\) *)
+
+(* (\* (\\* inline let lift_pure_state (a:Type) (wp:pure_wp a) (p:st_post a) (n:nat) = wp (fun a -> p a n) *\\) *\) *)
+(* (\* (\\* sub_effect PURE ~> STATE = lift_pure_state *\\) *\) *)
+(* (\* (\\* assume val r : range *\\) *\) *)
+
+(* (\* (\\* val repr_bind: #a:Type -> #b:Type -> #wp1:st_wp a -> #wp2:(a -> GTot (st_wp b)) *\\) *\) *)
+(* (\* (\\* 	     -> repr_STATE a wp1 *\\) *\) *)
+(* (\* (\\* 	     -> (x:a -> Tot (repr_STATE b (wp2 x))) *\\) *\) *)
+(* (\* (\\* 	     -> Tot (repr_STATE b (st_bind_wp nat r a b wp1 wp2)) *\\) *\) *)
+(* (\* (\\* #reset-options "--log_queries"	      *\\) *\) *)
+(* (\* (\\* let repr_bind #a #b #wp1 #wp2 f g =  *\\) *\) *)
+(* (\* (\\*   fun n0 -> admit(); //the encoding to SMT isn't sufficiently smart to capture monotonicity *\\) *\) *)
+(* (\* (\\*          let x, n1 = f n0 in *\\) *\) *)
+(* (\* (\\*          g x n1 *\\) *\) *)
 
 
 
